Refactoring of PDDL_Normalization.thy to use locales/contexts.

PDDL_Normalization.thy
@@ -1,429 +1,474 @@
 theory PDDL_Normalization
   imports "AI_Planning_Languages_Semantics.PDDL_STRIPS_Semantics"
-    Graph_Funs String_Shenanigans
+    Utils Graph_Funs String_Shenanigans
 begin
 
-text \<open>TODO: Even before performing normalization, we place a few restrictions on the input PDDL task.
-Some of these aren't strictly necessary and will only be kept in place for the MVP.\<close>
+subsection \<open> Input Restriction \<close>
+
+text \<open>Even before performing normalization, we place a few restrictions on the input PDDL task.
+Some of these aren't strictly necessary and will only be kept in place for the MVP:
+* Restrict consts/objects to primitive types only. This isn't strictly necessary but saves me a lot
+  of work, especially since I couldn't find any PDDL planning task that makes use of objects with
+  Either types. (domain and problem)
+* MVP: No disjunctions in goal formula: Our output format does not allow axioms, and I don't want
+  to generate auxiliary actions during normalization. (problem)
+* (maybe) check action signature types for well-formedness. (domain)\<close>
 
 text \<open>Check if a formula consists of only (nested) conjunctions of literals.\<close>
-fun only_conj :: "'a formula \<Rightarrow> bool" where
-  "only_conj (Atom a) \<longleftrightarrow> True" |
-  "only_conj \<bottom> \<longleftrightarrow> True" |
-  "only_conj (\<^bold>\<not> (Atom a)) \<longleftrightarrow> True" |
-  "only_conj (\<phi> \<^bold>\<and> \<psi>) \<longleftrightarrow> only_conj \<phi> \<and> only_conj \<psi>" |
-
-  "only_conj (\<^bold>\<not> _) \<longleftrightarrow> False" |
-  "only_conj (_ \<^bold>\<or> _) \<longleftrightarrow> False" |
-  "only_conj (_ \<^bold>\<rightarrow> _) \<longleftrightarrow> False"
-
-subsection \<open> Type Normalization \<close>
-abbreviation "type_names D \<equiv> remdups (''object'' # map fst (types D))"
-
 abbreviation singleton_types :: "('a \<times> type) list \<Rightarrow> bool" where
   "singleton_types os \<equiv> (\<forall>(_, t) \<in> set os. length (primitives t) = 1)"
 
-definition const_single_types :: "ast_domain \<Rightarrow> bool" where
-  "const_single_types D \<equiv> singleton_types (consts D)"
+context ast_domain
+begin
+  (* Omitting this from wf_action_schema is a little annoying for me *)
+  definition wf_action_params :: "ast_action_schema \<Rightarrow> bool" where
+    "wf_action_params a \<equiv> (\<forall>t \<in> snd ` (set (parameters a)). wf_type t)"
+  
+  definition restrict_dom :: bool where
+    "restrict_dom \<equiv> singleton_types (consts D)
+                    \<and> (\<forall>a\<in>set (actions D). wf_action_params a)"
+end
 
-definition objs_single_types :: "ast_problem \<Rightarrow> bool" where
-  ost_aux: "objs_single_types P \<equiv>
-    const_single_types (domain P)
-    \<and> singleton_types (objects P)"
+locale restr_domain = wf_ast_domain +
+  assumes restrD: restrict_dom
+begin
+  (* this is the most important and most referenced property restriction *)
+  lemma single_t_cnsts: "singleton_types (consts D)"
+    apply unfold_locales
+    using restrD by (auto simp add: restrict_dom_def)
+end
 
-definition restricted_pddl :: "ast_problem \<Rightarrow> bool" where
-  "restricted_pddl P \<longleftrightarrow> objs_single_types P"
+context ast_problem
+begin
+  definition restrict_prob :: bool where
+    "restrict_prob \<equiv> restrict_dom
+                  \<and> singleton_types (objects P)
+                  \<and> only_conj (goal P)"
+end
 
-definition pred_names :: "ast_domain \<Rightarrow> name list" where
-  "pred_names D = map (predicate.name \<circ> pred) (predicates D)"
+locale restr_prob = wf_ast_problem +
+  assumes restrP: restrict_prob
+begin
+  sublocale restr_domain "domain P"
+    apply unfold_locales
+    using restrP
+    unfolding restrict_prob_def by simp
 
-fun pred_for_type :: "ast_domain \<Rightarrow> name \<Rightarrow> predicate" where
-  "pred_for_type D t = Pred (safe_prefix (pred_names D) @ t)"
+  lemma single_t_cnsts: "singleton_types (objects P)"
+    apply unfold_locales
+    using restrP by (auto simp add: restrict_dom_def restrict_prob_def)
+end
 
-fun type_preds :: "ast_domain \<Rightarrow> predicate_decl list" where
-  "type_preds D = map ((\<lambda>p. PredDecl p [Either [''object'']]) \<circ> (pred_for_type D)) (type_names D)"
+subsection \<open>Type Normalization\<close>
 
-fun supertype_preds :: "ast_domain \<Rightarrow> name \<Rightarrow> predicate list" where
-  "supertype_preds D t = map (pred_for_type D) (reachable_nodes (types D) t)"
+(* TODO think of a better name *)
+abbreviation "\<omega> \<equiv> Either [''object'']"
 
-text \<open>This only works for singleton types on purpose.\<close>
-fun supertype_facts_for :: "ast_domain \<Rightarrow> (object \<times> type) \<Rightarrow> object atom formula list" where
-  "supertype_facts_for D (n, Either [t]) =
-    map (Atom \<circ> (\<lambda>p. predAtm p [n])) (supertype_preds D t)"
+context ast_domain
+begin
 
-fun type_conds :: "ast_domain \<Rightarrow> type \<Rightarrow> predicate list" where
-  "type_conds D (Either ts) = map (pred_for_type D) ts"
+  (* if multiple inheritance exists, there are duplicates *)
+  abbreviation "type_names \<equiv> remdups (''object'' # map fst (types D))"
+  
+  abbreviation pred_names :: "name list" where
+    "pred_names \<equiv> map (predicate.name \<circ> pred) (predicates D)"
+  
+  abbreviation pred_for_type :: "name \<Rightarrow> predicate" where
+    "pred_for_type t \<equiv> Pred (safe_prefix pred_names @ t)"
+  
+  definition type_preds :: "predicate_decl list" where
+    "type_preds \<equiv> map ((\<lambda>p. PredDecl p [\<omega>]) \<circ> pred_for_type) type_names"
 
-fun disj_fmlas :: "'a formula list \<Rightarrow> 'a formula" where
-  "disj_fmlas [] = Bot" |
-  "disj_fmlas [f] = f" |
-  "disj_fmlas (f # fs) = f \<^bold>\<or> disj_fmlas fs"
+  abbreviation supertypes_of :: "name \<Rightarrow> name list" where
+    "supertypes_of \<equiv> reachable_nodes (types D)"
 
-fun conj_fmlas :: "'a formula list \<Rightarrow> 'a formula" where
-  "conj_fmlas [] = \<^bold>\<not> \<bottom>" |
-  "conj_fmlas [f] = f" |
-  "conj_fmlas (f # fs) = f \<^bold>\<and> conj_fmlas fs"
+  definition supertype_preds :: "name \<Rightarrow> predicate list" where
+    "supertype_preds t \<equiv> map pred_for_type (supertypes_of t)"
+  
+  text \<open>This only works for singleton types on purpose.\<close>
+  fun supertype_facts_for :: "(object \<times> type) \<Rightarrow> object atom formula list" where
+    "supertype_facts_for (n, Either [t]) =
+      map (Atom \<circ> (\<lambda>p. predAtm p [n])) (supertype_preds t)" |
+    "supertype_facts_for (n, _) = undefined"
 
-fun type_precond :: "ast_domain \<Rightarrow> (variable \<times> type) \<Rightarrow> term atom formula" where
-  "type_precond D (v, T) =
-    disj_fmlas (map (Atom \<circ> (\<lambda>p. predAtm p [term.VAR v])) (type_conds D T))"
+  (* TODO sugar *)
+  fun type_conds :: "type \<Rightarrow> predicate list" where
+    "type_conds t = map pred_for_type (primitives t)"
+  
+  fun type_precond :: "(variable \<times> type) \<Rightarrow> term atom formula" where
+    "type_precond (v, T) =
+      disj_fmlas (map (Atom \<circ> (\<lambda>p. predAtm p [term.VAR v])) (type_conds T))"
+  
+  fun param_precond :: "(variable \<times> type) list \<Rightarrow> term atom formula" where
+    "param_precond params = conj_fmlas (map type_precond params)"
 
-fun param_precond :: "ast_domain \<Rightarrow> (variable \<times> type) list \<Rightarrow> term atom formula" where
-  "param_precond D params = conj_fmlas (map (type_precond D) params)"
+  abbreviation detype_pred :: "predicate_decl \<Rightarrow> predicate_decl" where
+    "detype_pred p \<equiv> PredDecl (pred p) (replicate (length (argTs p)) \<omega>)"
 
-fun detype_ent :: "('ent \<times> type) \<Rightarrow> ('ent \<times> type)" where
-  "detype_ent (n, T) = (n, Either [''object''])"
+  definition detype_preds :: "predicate_decl list \<Rightarrow> predicate_decl list" where
+    "detype_preds preds \<equiv> map detype_pred preds"
 
-definition detype_ents :: "('ent \<times> type) list \<Rightarrow> ('ent \<times> type) list" where
-  "detype_ents params \<equiv> map detype_ent params"
+  fun detype_ent :: "('ent \<times> type) \<Rightarrow> ('ent \<times> type)" where
+    "detype_ent (n, T) = (n, \<omega>)"
 
-fun detype_ac :: "ast_domain \<Rightarrow> ast_action_schema \<Rightarrow> ast_action_schema" where
-  "detype_ac D (Action_Schema nam params pre eff) =
-    Action_Schema nam (detype_ents params) (param_precond D params \<^bold>\<and> pre) eff"
+  definition detype_ents :: "('ent \<times> type) list \<Rightarrow> ('ent \<times> type) list" where
+    "detype_ents params \<equiv> map detype_ent params"
 
-fun detype_preds :: "predicate_decl list \<Rightarrow> predicate_decl list" where
-  "detype_preds preds =
-    map (\<lambda>pd. PredDecl (pred pd) (replicate (length (argTs pd)) (Either [''object'']))) preds"
+  fun detype_ac :: "ast_action_schema \<Rightarrow> ast_action_schema" where
+  "detype_ac (Action_Schema nam params pre eff) =
+    Action_Schema nam (detype_ents params) (param_precond params \<^bold>\<and> pre) eff"
+  (* TODO other alternative *)
+  lemma detype_ac_def:
+    "detype_ac ac = Action_Schema
+      (ast_action_schema.name ac)
+      (detype_ents (ast_action_schema.parameters ac))
+      (param_precond (ast_action_schema.parameters ac) \<^bold>\<and> (ast_action_schema.precondition ac))
+      (ast_action_schema.effect ac)"
+    by (metis ast_action_schema.collapse detype_ac.simps)
 
-fun detype_dom :: "ast_domain \<Rightarrow> ast_domain" where
-  "detype_dom D =
+  definition detype_dom :: "ast_domain" where
+  "detype_dom \<equiv>
     Domain
       []
-      (type_preds D @ detype_preds (predicates D))
+      (type_preds @ detype_preds (predicates D))
       (detype_ents (consts D))
-      (map (detype_ac D) (actions D))"
+      (map detype_ac (actions D))"
 
-fun supertype_facts :: "ast_domain \<Rightarrow> (object \<times> type) list \<Rightarrow> object atom formula list" where
-  "supertype_facts D objs = concat (map (supertype_facts_for D) objs)"
+  definition supertype_facts :: "(object \<times> type) list \<Rightarrow> object atom formula list" where
+    "supertype_facts objs \<equiv> concat (map supertype_facts_for objs)"
+end
 
-fun detype_prob :: "ast_problem \<Rightarrow> ast_problem" where
-  "detype_prob (Problem d objs i g) =
-    Problem
-      (detype_dom d)
-      (detype_ents objs)
-      (supertype_facts d objs @ supertype_facts d (consts d) @ i)
-      g"
+definition (in ast_problem) detype_prob :: "ast_problem" where
+"detype_prob \<equiv> Problem
+    detype_dom
+    (detype_ents (objects P))
+    (supertype_facts (objects P) @ supertype_facts (consts D) @ (init P))
+    (goal P)"
 
-definition typeless_dom :: "ast_domain \<Rightarrow> bool" where
-  "typeless_dom D = undefined"
+(*
+- type hierarchy is empty (implicitly includes ''object'')
+- predicate argument types are Either [''object'']
+- const types are Either [''object'']
+- actions parameters are detyped *)
+definition (in ast_domain) typeless_dom :: "bool" where
+  "typeless_dom \<equiv>
+    types D = []
+    \<and> (\<forall>p \<in> set (predicates D). \<forall>T \<in> set (argTs p). T = \<omega>)
+    \<and> undefined"
 
-definition typeless_prob :: "ast_problem \<Rightarrow> bool" where
-  "typeless_prob P = undefined"
+definition (in ast_problem) typeless_prob :: "bool" where
+  "typeless_prob \<equiv> typeless_dom \<and> undefined"
 
 subsection \<open>Complete Normalization\<close>
 
-definition normalized_prob :: "ast_problem \<Rightarrow> bool" where
-  "normalized_prob P \<equiv> typeless_prob P \<and> undefined"
+definition (in ast_problem) normalized_prob :: "bool" where
+  "normalized_prob \<equiv> typeless_prob \<and> undefined"
+
 
 (* ------------------------------------- PROOFS ------------------------------------------------- *)
 
-(* properties of Ab+La *)
+(* Properties of Ab+La *)
 
-lemma subtype_edge_swap: "ast_domain.subtype_edge = prod.swap"
-proof -
-  have "\<And>a b. ast_domain.subtype_edge (a, b) = prod.swap (a, b)"
-    by (simp add: ast_domain.subtype_edge.simps)
-  thus ?thesis by fast
-qed
+context ast_domain
+begin
+  
+  lemma subtype_edge_swap: "subtype_edge = prod.swap"
+  proof -
+    have "\<And>a b. subtype_edge (a, b) = prod.swap (a, b)"
+      by simp
+    thus ?thesis by fast
+  qed
+  
+  lemma wf_object: "ast_domain.wf_type d \<omega>"
+    unfolding ast_domain.wf_type.simps by simp
 
-lemma wf_object: "ast_domain.wf_type D (Either [''object''])"
-  unfolding ast_domain.wf_type.simps by simp
+  lemma tyterm_prop: "P (ty_term varT cnstT x) \<longleftrightarrow>
+    (case x of term.VAR x' \<Rightarrow> P (varT x') |
+               term.CONST x' \<Rightarrow> P (cnstT x'))"
+    apply (split term.split)
+    by simp
+  
+  lemma tyterm_elem: "(ty_term (map_of varT) (map_of cnstT) x \<noteq> None)
+    \<longleftrightarrow> (case x of term.VAR x' \<Rightarrow> x' \<in> fst ` set varT |
+                   term.CONST x' \<Rightarrow> x' \<in> fst ` set cnstT)"
+    apply (split term.split)
+    using tyterm_prop by (simp add: map_of_eq_None_iff)
 
-(* ty_term. I might be really bad at Isabelle*)
-lemma tyterm_simp: "(ty_term varT cnstT x) =
-  (case x of term.VAR x' \<Rightarrow> varT x' |
-                 term.CONST x' \<Rightarrow> cnstT x')"
-  apply (auto split: term.split)
-  done
+  (* signatures *)
+  
+  lemma sig_none: "sig p \<noteq> None \<longleftrightarrow> p \<in> pred ` set (predicates D)"
+  proof -
+    have "sig p = map_of (map (\<lambda>PredDecl p n \<Rightarrow> (p,n)) (predicates D)) p"
+      using sig_def by simp
+    have "sig p \<noteq> None \<longleftrightarrow> p \<in> fst ` set (map (\<lambda>PredDecl p n \<Rightarrow> (p, n)) (predicates D))"
+      by (metis map_of_eq_None_iff sig_def)
+    also have "... \<longleftrightarrow> p \<in> pred ` set (predicates D)"
+      by (simp add: image_iff predicate_decl.case_eq_if)
+    finally show ?thesis .
+  qed
+end
 
-lemma tyterm_prop: "P (ty_term varT cnstT x) \<longleftrightarrow>
-  (case x of term.VAR x' \<Rightarrow> P (varT x') |
-                 term.CONST x' \<Rightarrow> P (cnstT x'))"
-  by (metis tyterm_simp term.case_distrib)
+context wf_ast_domain
+begin
+  (* Deliberate shortcut: The goal is explaining that if a predatm in the original problem is well-
+  formed, so is the corresponding predatm in the detyped problem. I use distincness of predicate IDs
+  as an assumption here, to make the map_of logic simpler. But technically this isn't really
+  necessary. TODO explain, maybe *)
+  lemma pred_resolve:
+    shows "map_of (map (\<lambda>PredDecl p n \<Rightarrow> (p, n)) (predicates D)) p = Some Ts
+      \<longleftrightarrow> PredDecl p Ts \<in> set (predicates D)"
+  proof -
+    define preds where ps: "preds \<equiv> predicates D"
+    hence dis: "distinct (map pred preds)" using wf_domain wf_domain_def by simp
+    let ?map = "map (\<lambda>pd. (pred pd, argTs pd)) preds"
+    have zip: "?map = zip (map pred preds) (map argTs preds)"
+      by (induction preds) simp_all
+    hence "map_of ?map p = Some Ts \<longleftrightarrow> (p, Ts) \<in> set ?map" using dis by simp
+    also have "... \<longleftrightarrow> PredDecl p Ts \<in> set preds" by force
+    ultimately show ?thesis
+      by (simp add: predicate_decl.case_eq_if ps)
+  qed
 
-lemma tyterm_elem: "(ty_term (map_of varT) (map_of cnstT) x \<noteq> None)
-  \<longleftrightarrow> (case x of term.VAR x' \<Rightarrow> x' \<in> fst ` set varT |
-                 term.CONST x' \<Rightarrow> x' \<in> fst ` set cnstT)"
-proof -
-  have 1: "(ty_term (map_of varT) (map_of cnstT) x \<noteq> None)
-  \<longleftrightarrow> (case x of term.VAR x' \<Rightarrow> map_of varT x' \<noteq> None |
-                 term.CONST x' \<Rightarrow> map_of cnstT x' \<noteq> None)"
-    using tyterm_prop[where P = "\<lambda>x. x\<noteq>None"] by simp
-  thus ?thesis
-    using map_of_eq_None_iff[of cnstT] map_of_eq_None_iff[of varT] by presburger
-qed
+  lemma sig_some:
+    "sig p = Some Ts \<longleftrightarrow> PredDecl p Ts \<in> set (predicates D)"
+    using wf_domain wf_domain_def sig_def pred_resolve by presburger
 
-(* signatures *)
+  lemma sig_E:
+    assumes "sig p = Some Ts"
+    shows "\<exists>!i. i < length (predicates D) \<and> (predicates D ! i = PredDecl p Ts)"
+    oops
+end
 
-lemma sig_none: "ast_domain.sig D p \<noteq> None \<longleftrightarrow> p \<in> pred ` set (predicates D)"
-proof -
-  have "ast_domain.sig D p = map_of (map (\<lambda>PredDecl p n \<Rightarrow> (p,n)) (predicates D)) p"
-    using ast_domain.sig_def by simp
-  have "ast_domain.sig D p \<noteq> None \<longleftrightarrow>
-    map_of (map (\<lambda>PredDecl p n \<Rightarrow> (p, n)) (predicates D)) p \<noteq> None"
-    using ast_domain.sig_def by simp
-  also have "... \<longleftrightarrow> p \<in> fst ` set (map (\<lambda>PredDecl p n \<Rightarrow> (p, n)) (predicates D))"
-    by (metis map_of_eq_None_iff)
-  also have "... \<longleftrightarrow> p \<in> pred ` set (predicates D)"
-    by (simp add: image_iff predicate_decl.case_eq_if)
-  finally show ?thesis .
-qed
+context ast_domain begin
+  (* supertype enumeration *)
+  
+  lemma wf_type_iff_listed: "wf_type (Either ts) \<longleftrightarrow> (\<forall>t \<in> set ts. t \<in> set (type_names))"
+  proof -
+    have "set type_names = insert ''object'' (fst ` set (types D))"  by auto
+    thus ?thesis by (simp add: subset_code(1))
+  qed
 
-(* Deliberate shortcut: The goal is explaining that if a predatm in the original problem is well-
-formed, so is the corresponding predatm in the detyped problem. I use distincness of predicate IDs
-as an assumption here, to make the map_of logic simpler. But technically this isn't really
-necessary. TODO explain, maybe *)
-lemma pred_resolve:
-  assumes "distinct (map pred preds)"
-  shows "map_of (map (\<lambda>PredDecl p n \<Rightarrow> (p, n)) preds) p = Some Ts
-    \<longleftrightarrow> PredDecl p Ts \<in> set preds"
-proof -
-  let ?map = "map (\<lambda>P. (pred P, argTs P)) preds"
-  have zip: "?map = zip (map pred preds) (map argTs preds)"
-    by (induction preds) simp_all
-  hence "map_of ?map p = Some Ts \<longleftrightarrow> (p, Ts) \<in> set ?map" using assms by simp
-  also have "... \<longleftrightarrow> PredDecl p Ts \<in> set preds" by force
-  ultimately show ?thesis
-    by (simp add: predicate_decl.case_eq_if)
-qed
+  lemma of_type_iff_reach:
+    shows "of_type oT T \<longleftrightarrow> (
+      \<forall>ot \<in> set (primitives oT).
+      \<exists>t \<in> set (primitives T).
+        t \<in> set (supertypes_of ot))"
+  proof -
+    have "subtype_rel = set (map prod.swap (types D))"
+      using subtype_rel_def subtype_edge_swap by metis
+    hence subrel_inv: "subtype_rel = (set (types D))\<inverse>" by auto
+    hence "of_type oT T \<longleftrightarrow>
+      set (primitives oT) \<subseteq> ((set (types D))\<inverse>)\<^sup>* `` set (primitives T)"
+      using of_type_def by simp
+    also have "... \<longleftrightarrow>
+      set (primitives oT) \<subseteq> ((set (types D))\<^sup>*)\<inverse> `` set (primitives T)"
+      by (simp add: rtrancl_converse)
+    also have "... \<longleftrightarrow>
+      (\<forall>ot \<in> set (primitives oT). ot \<in> ((set (types D))\<^sup>*)\<inverse> `` set (primitives T))"
+      by auto
+    also have "... \<longleftrightarrow>
+      (\<forall>ot \<in> set (primitives oT). \<exists>t. (ot, t) \<in> (set (types D))\<^sup>* \<and> t \<in> set (primitives T))"
+      by auto
+    finally show ?thesis using reachable_iff_in_star by metis
+  qed
+end
 
-lemma sig_some:
-  assumes "distinct (map pred (predicates D))"
-  shows "ast_domain.sig D p = Some Ts \<longleftrightarrow> PredDecl p Ts \<in> set (predicates D)"
-  using assms ast_domain.sig_def pred_resolve by presburger
 
-lemma sig_E:
-  assumes "ast_domain.sig D p = Some Ts"
-  obtains i where "i < length (predicates D)" "predicates D ! i = PredDecl p Ts"
-  oops
-
-(* supertype enumeration *)
-
-lemma wf_type_iff_listed: "ast_domain.wf_type D (Either ts) \<longleftrightarrow> (\<forall>t \<in> set ts. t \<in> set (type_names D))"
-proof -
-  have "set (type_names D) = insert ''object'' (fst ` set (types D))" by auto
-  thus ?thesis by (simp add: ast_domain.wf_type.simps subset_code(1))
-qed
-
-lemma of_type_iff_reach:
-  shows "ast_domain.of_type D oT T \<longleftrightarrow> (
-    \<forall>ot \<in> set (primitives oT).
-    \<exists>t \<in> set (primitives T).
-      t \<in> set (reachable_nodes (types D) ot))"
-proof -
-  have "ast_domain.subtype_rel D = set (map prod.swap (types D))"
-    using ast_domain.subtype_rel_def subtype_edge_swap by metis
-  hence subrel_inv: "ast_domain.subtype_rel D = (set (types D))\<inverse>" by auto
-  hence "ast_domain.of_type D oT T \<longleftrightarrow>
-    set (primitives oT) \<subseteq> ((set (types D))\<inverse>)\<^sup>* `` set (primitives T)"
-    using ast_domain.of_type_def by simp
-  also have "... \<longleftrightarrow>
-    set (primitives oT) \<subseteq> ((set (types D))\<^sup>*)\<inverse> `` set (primitives T)"
-    by (simp add: rtrancl_converse)
-  also have "... \<longleftrightarrow>
-    (\<forall>ot \<in> set (primitives oT). ot \<in> ((set (types D))\<^sup>*)\<inverse> `` set (primitives T))" by auto
-  also have "... \<longleftrightarrow>
-    (\<forall>ot \<in> set (primitives oT). \<exists>t. (ot, t) \<in> (set (types D))\<^sup>* \<and> t \<in> set (primitives T))" by auto
-  finally show ?thesis using reachable_iff_in_star by metis
-qed
-
-lemma obj_of_type_iff_reach:
-  assumes "ast_problem.objT P n = Some oT"
-  shows  "ast_problem.is_obj_of_type P n T \<longleftrightarrow>
+lemma (in ast_problem) obj_of_type_iff_reach:
+  assumes "objT n = Some oT"
+  shows  "is_obj_of_type n T \<longleftrightarrow>
     (\<forall>ot \<in> set (primitives oT).
       \<exists>t \<in> set (primitives T).
-    t \<in> set (reachable_nodes (types (domain P)) ot))"
-  using assms ast_problem.is_obj_of_type_def of_type_iff_reach by auto
+    t \<in> set (supertypes_of ot))"
+  using assms is_obj_of_type_def of_type_iff_reach by auto
 
-lemma single_of_type_iff:
-  shows "ast_domain.of_type D (Either [ot]) T \<longleftrightarrow> (
+lemma (in ast_domain) single_of_type_iff:
+  shows "of_type (Either [ot]) T \<longleftrightarrow> (
     \<exists>t \<in> set (primitives T).
-      t \<in> set (reachable_nodes (types D) ot))"
+      t \<in> set (supertypes_of ot))"
   using of_type_iff_reach by simp
 
-lemma simple_obj_of_type_iff:
-  assumes "ast_problem.objT P n = Some (Either [ot])"
-  shows  "ast_problem.is_obj_of_type P n T \<longleftrightarrow>
+lemma (in ast_problem) simple_obj_of_type_iff:
+  assumes "objT n = Some (Either [ot])"
+  shows  "is_obj_of_type n T \<longleftrightarrow>
       (\<exists>t \<in> set (primitives T).
-    t \<in> set (reachable_nodes (types (domain P)) ot))"
-  using assms ast_problem.is_obj_of_type_def single_of_type_iff by auto
+    t \<in> set (supertypes_of ot))"
+  using assms is_obj_of_type_def single_of_type_iff by auto
 
-(* type normalization well-formed *)
-lemma dist_prefix: "distinct xs \<Longrightarrow> distinct (map ((@) (safe_prefix ys)) xs)"
-  by (simp add: distinct_conv_nth)
-lemma dist_pred: "distinct xs \<Longrightarrow> distinct (map Pred xs)"
+subsubsection \<open> Type Normalization Produces Typeless PDDL \<close>
+
+(* TODO *)
+
+subsubsection \<open> Type Normalization Preserves Well-Formedness \<close>
+
+lemma dist_pred: "distinct names \<Longrightarrow> distinct (map Pred names)"
   by (meson distinct_map inj_onI predicate.inject)
 
-lemma t_preds_names: (* TODO simplify *)
-  assumes "distinct (map pred (predicates D))"
-  shows "distinct (map pred (type_preds D @ detype_preds (predicates D)))"
-proof -
-  (* Predicate names are unique because the original predicate names are unchanged
-     and the additional predicate names are unique (based on unique type names)
-     and distinct from the original predicates. *)
-  let ?preds = "map pred (predicates D)"
-  let ?t_preds = "map pred (type_preds D)"
-  let ?dt_preds = "map pred (detype_preds (predicates D))"
+context wf_ast_domain
+begin
+  lemmas wf_dom_def = wf_domain[unfolded wf_domain_def]
 
-  have p_eq_dt: "?preds = ?dt_preds" by simp
-  hence g1: "distinct ( map pred (detype_preds (predicates D)))"
-    using assms by argo
+  lemma (in ast_domain) t_pred_name: "pred pd = pred (detype_pred pd)" by simp
 
-  let ?prefix = "safe_prefix (map predicate.name ?preds)"
-  (* =  map (pred_for_type D) (type_names D) *)
-  have dist_types: "distinct (type_names D)" by auto
-  have t_ps_expand: "?t_preds = map (Pred \<circ> ((@) ?prefix)) (type_names D)"
-    by (simp add: pred_names_def)
-  (* define, not let, because the terms become too big for the solver *)
-  define pnames where "pnames \<equiv> map predicate.name ?preds"
-  define tp_names where "tp_names \<equiv> map (((@) (safe_prefix pnames))) (type_names D)"
+  lemma t_preds_names: (* TODO simplify *)
+    shows "distinct (map pred (predicates detype_dom))"
+  proof -
+    (* Predicate names are unique because the original predicate names are unchanged
+       and the additional predicate names are unique (based on unique type names)
+       and distinct from the original predicates. *)
+    let ?preds = "map pred (predicates D)"
+    let ?t_preds = "map pred type_preds"
+    let ?dt_preds = "map pred (detype_preds (predicates D))"
+
+    have dis: "distinct (map pred (predicates D))" using wf_dom_def by simp
+    have p_eq_dt: "?preds = ?dt_preds" using t_pred_name detype_preds_def by simp
+    hence g1: "distinct ( map pred (detype_preds (predicates D)))"
+      using dis by argo
   
-  have "set (map ((@) (safe_prefix pnames)) (type_names D)) \<inter> set pnames = {}"
-    using safe_prefix_correct by auto
-  hence "set tp_names \<inter> set pnames = {}" using tp_names_def pnames_def by simp
-  hence "set (map Pred tp_names) \<inter> set (map Pred pnames) = {}" by auto
-  hence "set (map (Pred \<circ> ((@) (safe_prefix pnames))) (type_names D)) \<inter> set (map Pred pnames) = {}"
-    using tp_names_def by (metis map_map)
-
-  moreover have "map Pred pnames = ?preds" using pnames_def by simp
-  moreover have "?t_preds = map (Pred \<circ> ((@) (safe_prefix pnames))) (type_names D)"
-    using t_ps_expand pnames_def by blast
-  ultimately have g2: "set ?t_preds \<inter> set ?dt_preds = {}" by (metis p_eq_dt)
+    let ?prefix = "safe_prefix (map predicate.name ?preds)"
+    (* =  map (pred_for_type D) (type_names D) *)
+    have t_ps_expand: "?t_preds = map (Pred \<circ> ((@) ?prefix)) type_names"
+      by (simp add: type_preds_def)
+    (* define, not let, because the terms become too big for the solver *)
+    define pnames where "pnames \<equiv> map predicate.name ?preds"
+    define tp_names where "tp_names \<equiv> map (((@) (safe_prefix pnames))) type_names"
+    
+    have "set (map ((@) (safe_prefix pnames)) type_names) \<inter> set pnames = {}"
+      using safe_prefix_correct by auto
+    hence "set tp_names \<inter> set pnames = {}" using tp_names_def pnames_def by simp
+    hence "set (map Pred tp_names) \<inter> set (map Pred pnames) = {}" by auto
+    hence "set (map (Pred \<circ> ((@) (safe_prefix pnames))) type_names) \<inter> set (map Pred pnames) = {}"
+      using tp_names_def by (metis map_map)
   
-  have d: "distinct (map ((@) ?prefix) (type_names D))"
-    using dist_prefix dist_types by simp
-  hence "distinct (map (Pred \<circ> ((@) ?prefix)) (type_names D))"
-    using dist_pred[OF d] by simp
-  hence g3: "distinct (?t_preds)" using t_ps_expand by metis
-
-  from g1 g2 g3 show ?thesis by simp
-qed
-
-lemma t_preds_names2:
-  assumes "distinct (map pred (predicates D))"
-  shows "distinct (map pred (predicates (detype_dom D)))"
-  using assms
-  using t_preds_names ast_domain.sel(2) detype_dom.simps by presburger
-
-lemma t_preds_wf:
-  "\<forall>p \<in> set (type_preds D @ (detype_preds (predicates D))).
-    ast_domain.wf_predicate_decl (detype_dom D) p"
-  (is "\<forall>p \<in> ?s. ?wf p")
-proof -
-  let ?D2 = "detype_dom D"
-  have c1: "\<forall>p \<in> set (type_preds D). ?wf p"
-  proof
-    fix p assume "p \<in> set (type_preds D)"
-    hence "\<forall>t \<in> set (argTs p). ast_domain.wf_type ?D2 t" using wf_object by auto
-    thus "?wf p"
-      by (metis ast_domain.wf_predicate_decl.simps predicate_decl.exhaust_sel)
+    moreover have "map Pred pnames = ?preds" using pnames_def by simp
+    moreover have "?t_preds = map (Pred \<circ> ((@) (safe_prefix pnames))) type_names"
+      using t_ps_expand pnames_def by blast
+    ultimately have g2: "set ?t_preds \<inter> set ?dt_preds = {}" by (metis p_eq_dt)
+    
+    have d: "distinct (map ((@) ?prefix) type_names)" (* fact: distinct type_names *)
+      using dist_prefix by simp
+    hence "distinct (map (Pred \<circ> ((@) ?prefix)) type_names)"
+      using dist_pred[OF d] by simp
+    hence g3: "distinct (?t_preds)" using t_ps_expand by metis
+  
+    from g1 g2 g3 have "distinct (map pred (type_preds @ detype_preds (predicates D)))" by simp
+    thus ?thesis using ast_domain.sel(2) detype_dom_def by presburger
   qed
-  have c2: "\<forall>p \<in> set (detype_preds (predicates D)). ?wf p"
-  proof
-    fix p assume "p \<in> set (detype_preds (predicates D))"
-    hence "\<forall>t \<in> set (argTs p). t = Either [''object'']" by auto
-    hence "\<forall>t \<in> set (argTs p). ast_domain.wf_type ?D2 t" using wf_object by auto
-    thus "?wf p"
-      by (metis ast_domain.wf_predicate_decl.simps predicate_decl.exhaust_sel)
+
+  lemma (in ast_domain) t_preds_wf:
+    "\<forall>p \<in> set (type_preds @ (detype_preds (predicates D))).
+      ast_domain.wf_predicate_decl detype_dom p"
+    (is "\<forall>p \<in> ?s. ?wfp2 p")
+  proof -
+    interpret d2 : ast_domain "detype_dom" . (* how to just do this everywhere in the context? *)
+    have c1: "\<forall>p \<in> set type_preds. d2.wf_predicate_decl p"
+    proof
+      fix p assume "p \<in> set type_preds"
+      hence "\<forall>t \<in> set (argTs p). t = \<omega>" using type_preds_def by auto
+      hence "\<forall>t \<in> set (argTs p). d2.wf_type t"
+        using wf_object d2.wf_object by fastforce
+      thus "?wfp2 p"
+        by (metis d2.wf_predicate_decl.simps predicate_decl.exhaust_sel)
+    qed
+    have c2: "\<forall>p \<in> set (detype_preds (predicates D)). ?wfp2 p"
+    proof
+      fix p assume "p \<in> set (detype_preds (predicates D))"
+      hence "\<forall>t \<in> set (argTs p). t = \<omega>" using detype_preds_def by auto
+      hence "\<forall>t \<in> set (argTs p). d2.wf_type t" using wf_object by auto
+      thus "?wfp2 p"
+        by (metis d2.wf_predicate_decl.simps predicate_decl.exhaust_sel)
+    qed
+    (* just to speed things up *)
+    thus ?thesis using c1 c2 by auto
   qed
-  (* just to speed things up *)
-  have "\<And>xs ys P. \<forall>x \<in> set xs. P x \<Longrightarrow> \<forall>y \<in> set ys. P y \<Longrightarrow> \<forall>x' \<in> set (xs @ ys). P x'"
-    by auto
-  note this[OF c1 c2] thus ?thesis .
-qed
 
-lemma t_ents_names:
-  assumes "distinct (map fst ents)"
-  shows "distinct (map fst (detype_ents ents))"
-proof -
-  have "\<And>xs. map fst xs = map fst (map detype_ent xs)" by auto
-  thus ?thesis using assms by (metis detype_ents_def)
-qed
+  lemma (in ast_domain) t_ents_names:
+    assumes "distinct (map fst ents)"
+    shows "distinct (map fst (detype_ents ents))"
+  proof -
+    have "\<And>xs. map fst xs = map fst (map detype_ent xs)" by auto
+    thus ?thesis using assms by (metis detype_ents_def)
+  qed
 
-(* did I mess up simp somehow? why is this getting harder? *)
-lemma t_ents_wf_aux:
-  shows "(\<forall>ent\<in>set (detype_ents ents). ast_domain.wf_type (detype_dom D) (snd ent))"
-proof
-  fix ent assume elem: "ent \<in> set (detype_ents ents)"
-  obtain n T where nT: "(n, T) = ent" by (metis surjective_pairing)
+  (* did I mess up simp somehow? why is this getting harder? *)
+  lemma (in ast_domain) t_ents_wf_aux:
+    shows "(\<forall>ent\<in>set (detype_ents ents). ast_domain.wf_type detype_dom (snd ent))"
+  proof
+    interpret d2 : ast_domain detype_dom .
+    fix ent assume elem: "ent \<in> set (detype_ents ents)"
+    obtain n T where nT: "(n, T) = ent" by (metis surjective_pairing)
 
-  from elem nT obtain og where "og \<in> set ents" and 2: "ent = detype_ent og"
-    by (metis (mono_tags, lifting) detype_ents_def image_iff list.set_map)
-  from nT 2 have "T = Either [''object'']" by (metis detype_ent.elims prod.inject)
-  hence "ast_domain.wf_type (detype_dom D) T" using wf_object by simp
-  thus "ast_domain.wf_type (detype_dom D) (snd ent)" using nT by fastforce
-qed
+    from elem nT obtain og where "og \<in> set ents" and 2: "ent = detype_ent og"
+      by (metis (mono_tags, lifting) detype_ents_def image_iff list.set_map)
+    from nT 2 have "T = \<omega>" by (metis detype_ent.elims prod.inject)
+    hence "d2.wf_type T" using wf_object by simp
+    thus "d2.wf_type (snd ent)" using nT by fastforce
+  qed
 
-lemma t_ents_wf:
-  shows "(\<forall>(n,T)\<in>set (detype_ents ents). ast_domain.wf_type (detype_dom D) T)"
-  using t_ents_wf_aux by fastforce
+  lemma (in ast_domain) t_ents_wf:
+    shows "(\<forall>(n,T)\<in>set (detype_ents ents). ast_domain.wf_type detype_dom T)"
+    using t_ents_wf_aux by fastforce
 
 (* formulas *)
 
 (* Detyped formulas *)
 
-lemma
-  "map (\<lambda>t. y) xs = replicate (length xs) y"
-  by (simp add: map_replicate_const)
+  lemma
+    assumes "sig p = Some Ts"
+    shows "ast_domain.sig detype_dom p
+      = Some (replicate (length Ts) \<omega>)"
+  proof -
+    have "distinct (map pred (predicates D))" using wf_dom_def by simp
+    hence "PredDecl p Ts \<in> set (predicates D)" using assms sig_some by blast
+    have "predicates detype_dom = type_preds @
+      map (\<lambda>pd. PredDecl (pred pd) (replicate (length (argTs pd)) \<omega>)) (predicates D)"
+      using detype_dom_def detype_preds_def by simp
+    from assms have "distinct (map pred (predicates detype_dom))"
+      using t_preds_names by simp
+    oops
 
-(* pred sig ts \<Longrightarrow> detype pred sig (detype ts)*)
-lemma
-  assumes "distinct (map pred (predicates D))"
-  assumes "ast_domain.sig D p = Some Ts"
-  shows "ast_domain.sig (detype_dom D) p
-    = Some (replicate (length Ts) (Either [''object'']))"
-proof -
-  from assms have "PredDecl p Ts \<in> set (predicates D)" using sig_some by blast
-  have "predicates (detype_dom D) =
-    map (\<lambda>pd. PredDecl (pred pd) (replicate (length (argTs pd)) (Either [''object'']))) (predicates D)"
-  oops
-
-
-
-
-(* ty_term (map_of params) constT *)
-
-(* fun wf_pred_atom_c :: "ast_domain \<Rightarrow> ('ent \<rightharpoonup> type) \<Rightarrow> predicate \<times> 'ent list \<Rightarrow> bool" where
-  "wf_pred_atom_c D ty_ent (p,vs) \<longleftrightarrow> (
-    case (sig_c D) p of
-      None \<Rightarrow> False
-    | Some Ts \<Rightarrow> list_all2 (is_of_type_c D ty_ent) vs Ts)" *)
-
-(* I feel like I need to figure out how to make my formulas smaller *)
-lemma
-  assumes "ast_domain.wf_pred_atom D (ty_term (map_of params) (ast_domain.constT D )) (p,vs)"
-  defines "D2 \<equiv> (detype_dom D)"
-  shows "ast_domain.wf_pred_atom D2 (ty_term (map_of (detype_ents params)) (ast_domain.constT D2)) (p,vs)"
-proof -
-  let ?tyt = "ty_term (map_of params) (ast_domain.constT D )"
-  let ?tyt2 = "ty_term (map_of (detype_ents params)) (ast_domain.constT D2)"
-  
-  from assms obtain Ts where "ast_domain.sig D p = Some Ts \<and> list_all2 (ast_domain.is_of_type D ?tyt) vs Ts"
-    by (metis not_None_eq option.simps(4-5) ast_domain.wf_pred_atom.simps)
-  hence "length vs = length Ts" using list_all2_lengthD by auto
+  (* I feel like I need to figure out how to make my formulas smaller *)
+  lemma (in ast_domain)
+    assumes "wf_pred_atom (ty_term (map_of params) constT) (p,vs)"
+    defines "D2 \<equiv> detype_dom"
+    shows "ast_domain.wf_pred_atom D2 (ty_term (map_of (detype_ents params)) (ast_domain.constT D2)) (p,vs)"
+  proof -
+    interpret d2 : ast_domain detype_dom .
+    let ?tyt = "ty_term (map_of params) constT"
+    let ?tyt2 = "ty_term (map_of (detype_ents params)) d2.constT"
+    
+    from assms obtain Ts where "sig p = Some Ts \<and> list_all2 (is_of_type ?tyt) vs Ts"
+      by (metis not_None_eq option.simps(4-5) wf_pred_atom.simps)
+    hence "length vs = length Ts" using list_all2_lengthD by auto
+    oops
 
 
+  (* ty_term (map_of params) constT *)
 
-  oops
+  (* fun wf_pred_atom_c :: "ast_domain \<Rightarrow> ('ent \<rightharpoonup> type) \<Rightarrow> predicate \<times> 'ent list \<Rightarrow> bool" where
+    "wf_pred_atom_c D ty_ent (p,vs) \<longleftrightarrow> (
+      case (sig_c D) p of
+        None \<Rightarrow> False
+      | Some Ts \<Rightarrow> list_all2 (is_of_type_c D ty_ent) vs Ts)" *)
 
-(* actions *)
+  (* actions *)
+  abbreviation (in ast_domain) "ac_name \<equiv> ast_action_schema.name"
+  (* abbreviation (in ast_domain) "ac_params \<equiv> ast_action_schema.parameters" -- just use \<open>parameters\<close> *)
+  abbreviation (in ast_domain) "ac_pre \<equiv> ast_action_schema.precondition"
+  abbreviation (in ast_domain) "ac_eff \<equiv> ast_action_schema.effect"
 
+  lemma t_acs_names:
+    shows "distinct (map ac_name (map detype_ac (actions D)))"
+  proof -
+    have dis: "distinct (map ac_name (actions D))"
+      using wf_dom_def by simp
+    have "map ac_name (actions D) = map ac_name (map detype_ac (actions D))"
+      by (simp add: detype_ac_def)
+    thus ?thesis using dis by argo
+  qed
 
-
-lemma t_acs_names:
-  assumes "distinct (map ast_action_schema.name (actions D))"
-  shows "distinct (map ast_action_schema.name (map (detype_ac D) (actions D)))"
-proof -
-  have "\<And>ac. ast_action_schema.name ac = ast_action_schema.name (detype_ac D ac)"
-    by (metis ast_action_schema.collapse ast_action_schema.sel(1) detype_ac.simps)
-  (* I'd like composition syntax but the automatic solver doesn't like me today *)
-  hence "map ast_action_schema.name (actions D) = map ast_action_schema.name (map (detype_ac D) (actions D))"
-    by simp
-  thus ?thesis using assms by argo
-qed
-
-(* wf type not checked! *)
-(* fun wf_action_schema :: "ast_action_schema \<Rightarrow> bool" where
+  (* wf type not checked! *)
+  (* fun wf_action_schema :: "ast_action_schema \<Rightarrow> bool" where
     "wf_action_schema (Action_Schema n params pre eff) \<longleftrightarrow> (
       let
         tyt = ty_term (map_of params) constT
@@ -432,93 +477,83 @@ qed
       \<and> wf_fmla tyt pre
       \<and> wf_effect tyt eff)" *)
 
-lemma "\<forall>x \<in> set xs. P x \<Longrightarrow> \<forall>x. P x \<longrightarrow> Q (f x) \<Longrightarrow> \<forall>x \<in> set (map f xs). Q x"
-  by simp
-
-lemma wf_ac_expanded: "ast_domain.wf_action_schema D a \<longleftrightarrow> (
+  (* TODO just manipulate lemma  *)
+  lemma (in ast_domain) wf_ac_expanded:
+    "wf_action_schema a \<longleftrightarrow> (
       let
-        tyt = ty_term (map_of (parameters a)) (ast_domain.constT D)
+        tyt = ty_term (map_of (parameters a)) constT
       in
         distinct (map fst (parameters a))
-      \<and> ast_domain.wf_fmla D tyt (ast_action_schema.precondition a)
-      \<and> ast_domain.wf_effect D tyt (ast_action_schema.effect a))"
-  using ast_domain.wf_action_schema.simps
-  by (metis ast_action_schema.collapse)
+      \<and> wf_fmla tyt (ac_pre a)
+      \<and> wf_effect tyt (ac_eff a))"
+    using wf_action_schema.simps
+    by (metis ast_action_schema.collapse)
 
-lemma t_acs_wf_aux:
-  assumes "ast_domain.wf_action_schema D a"
-  shows "ast_domain.wf_action_schema (detype_dom D) (detype_ac D a)"
-proof -
-  let ?D2 = "detype_dom D"
-  let ?a2 = "detype_ac D a"
-  define tyt where tyt: "tyt \<equiv> ty_term (map_of (parameters a)) (ast_domain.constT D)"
-  from assms have 1: "distinct (map fst (parameters a))" using wf_ac_expanded by metis
-  from assms tyt have 2: "ast_domain.wf_fmla D tyt (ast_action_schema.precondition a)" using wf_ac_expanded by metis
-  from assms tyt have 3: "ast_domain.wf_effect D tyt (ast_action_schema.effect a)" using wf_ac_expanded by metis
-
-  define tyt2 where tyt2: "tyt2 \<equiv> ty_term (map_of (parameters ?a2)) (ast_domain.constT ?D2)"
-  have ps: "parameters ?a2 = detype_ents (parameters a)"
-    by (metis ast_action_schema.collapse ast_action_schema.sel(2) detype_ac.simps)
-  hence c1: "distinct (map fst (parameters ?a2))" using 1 t_ents_names by auto
-  from ps have cx: "(\<forall>(n,T)\<in>set (parameters ?a2). ast_domain.wf_type (detype_dom D) T)"
-    using t_ents_wf by metis (* not required for wf_action_schema but should be, maybe *)
-
-  have c2a: "ast_domain.wf_fmla ?D2 tyt2 (param_precond D (parameters a))" sorry
-  have c2b: "ast_domain.wf_fmla ?D2 tyt2 (ast_action_schema.precondition a)" sorry
-  from c2a c2b have c2: "ast_domain.wf_fmla ?D2 tyt2 (ast_action_schema.precondition ?a2)"
-    by (metis ast_action_schema.collapse ast_action_schema.sel(3) ast_domain.wf_fmla.simps(3) detype_ac.simps)
-  have "ast_domain.wf_effect ?D2 tyt2 (ast_action_schema.effect a)" sorry
-  hence c3: "ast_domain.wf_effect ?D2 tyt2 (ast_action_schema.effect ?a2)"
-    by (metis ast_action_schema.collapse ast_action_schema.sel(4) detype_ac.simps)
-
-  from c1 c2 c3 tyt2 show ?thesis using wf_ac_expanded by auto
-qed
-
-lemma t_acs_wf:
-  assumes "\<forall>a\<in>set (actions D). ast_domain.wf_action_schema D a"
-  shows "(\<forall>a\<in>set (map (detype_ac D) (actions D)). ast_domain.wf_action_schema (detype_dom D) a)"
-  oops
+  lemma (in ast_domain) t_acs_wf_aux:
+    assumes "wf_action_schema a"
+    shows "ast_domain.wf_action_schema detype_dom (detype_ac a)"
+  proof -
+    interpret d2 : ast_domain detype_dom .
+    let ?a2 = "detype_ac a"
+    define tyt where tyt: "tyt \<equiv> ty_term (map_of (parameters a)) constT"
+    from assms have 1: "distinct (map fst (parameters a))" using wf_ac_expanded by metis
+    from assms tyt have 2: "wf_fmla tyt (ac_pre a)" using wf_ac_expanded by metis
+    from assms tyt have 3: "wf_effect tyt (ac_eff a)" using wf_ac_expanded by metis
   
+    define tyt2 where tyt2: "tyt2 \<equiv> ty_term (map_of (parameters ?a2)) d2.constT"
+    have ps: "parameters ?a2 = detype_ents (parameters a)" by (simp add: detype_ac_def)
+    hence c1: "distinct (map fst (parameters ?a2))" using 1 t_ents_names by auto
+    text \<open>This fact is not required for \<open>wf_action_schema\<close> but it should be, maybe\<close>
+    from ps have cx: "(\<forall>(n,T)\<in>set (parameters ?a2). d2.wf_type T)"
+      using t_ents_wf by metis
+  
+    have c2a: "d2.wf_fmla tyt2 (param_precond (parameters a))" sorry
+    have c2b: "d2.wf_fmla tyt2 (ac_pre a)" sorry
+    from c2a c2b have c2: "d2.wf_fmla tyt2 (ac_pre ?a2)" by (simp add: detype_ac_def)
+    have "d2.wf_effect tyt2 (ac_eff a)" sorry
+    hence c3: "d2.wf_effect tyt2 (ac_eff ?a2)" by (simp add: detype_ac_def)
+  
+    from c1 c2 c3 tyt2 show ?thesis using d2.wf_ac_expanded by simp
+  qed
 
-theorem detype_dom_wf:
-  assumes "ast_domain.wf_domain D"
-  shows "ast_domain.wf_domain (detype_dom D)"
-proof -
-  let ?D2 = "detype_dom D"
-  from assms have
-    typs: "ast_domain.wf_types D" and
-    pred_names: "distinct (map pred (predicates D))" and
-    wf_preds: "\<forall>p\<in>set (predicates D). ast_domain.wf_predicate_decl D p" and
-    cnst_names: "distinct (map fst (consts D))" and
-    wf_cnsts: "\<forall>(n,T)\<in>set (consts D). ast_domain.wf_type D T" and
-    ac_names: "distinct (map ast_action_schema.name (actions D))" and
-    wf_acs: "\<forall>a\<in>set (actions D). ast_domain.wf_action_schema D a"
-    by (simp_all add: ast_domain.wf_domain_def)
+  lemma t_acs_wf:
+    shows "(\<forall>a\<in>set (map detype_ac (actions D)). ast_domain.wf_action_schema detype_dom a)"
+  proof -
+    interpret d2 : ast_domain detype_dom .
+    have wf_acs: "\<forall>a\<in>set (actions D). wf_action_schema a" using wf_dom_def by simp
+    oops
 
-  (* Types are well-formed because they are simply empty. *)
-  have c1: "ast_domain.wf_types ?D2" using ast_domain.wf_types_def by simp
-  note c2 = t_preds_names[OF pred_names]
-  note c3 = t_preds_wf
-  have c4: "distinct (map fst (detype_ents(consts D)))"
-    using cnst_names by (simp add: t_ents_names)
-  have c5: "(\<forall>(n,T)\<in>set (detype_ents (consts D)). ast_domain.wf_type ?D2 T)"
-    using wf_cnsts t_ents_wf by metis
-  have c6: "distinct (map ast_action_schema.name (map (detype_ac D) (actions D)))"
-    using ac_names t_acs_names by simp
-  have c7: "(\<forall>a\<in>set (map (detype_ac D) (actions D)). ast_domain.wf_action_schema ?D2 a)" sorry
+  theorem detype_dom_wf:
+    shows "ast_domain.wf_domain detype_dom"
+  proof -
+    interpret d2 : ast_domain detype_dom .
+  
+    (* Types are well-formed because they are simply empty. *)
+    have c1: "d2.wf_types" using d2.wf_types_def detype_dom_def by simp
+    note c2 = t_preds_names
+    note c3 = t_preds_wf
+    have "distinct (map fst (consts D))" using wf_dom_def by simp
+    hence c4: "distinct (map fst (detype_ents(consts D)))"
+      by (simp add: t_ents_names)
+    have c5: "(\<forall>(n,T)\<in>set (detype_ents (consts D)). d2.wf_type T)"
+      using t_ents_wf by metis
+    have c6: "distinct (map ac_name (map detype_ac (actions D)))"
+      using t_acs_names by simp
+    have c7: "(\<forall>a\<in>set (map detype_ac (actions D)). d2.wf_action_schema a)" sorry
+  
+    from c1 c2 c3 c4 c5 c6 c7 show ?thesis
+      using d2.wf_domain_def detype_dom_def by simp
+  qed
 
-  from c1 c2 c3 c4 c5 c6 c7 show ?thesis
-    using ast_domain.wf_domain_def by auto
-qed
-
-lemma "distinct nams \<Longrightarrow> distinct (map Pred nams)"
-  by (meson distinct_map inj_onI predicate.inject)
-
+end
 
 lemma "set as \<inter> set bs = {} \<Longrightarrow> distinct as \<Longrightarrow> distinct bs \<Longrightarrow> distinct (as @ bs)"
   by simp
 
+(* ---------------------- Milestones ------------------------- *)
 
+
+(* TODO update locale hierarchy accordingly *)
 lemma "ast_problem.wf_problem P \<Longrightarrow> ast_problem.wf_problem (detype_prob P)"
   oops
 
